\documentclass[article]{journal}
\usepackage{amsmath,amssymb}
\usepackage{bussproofs}
\usepackage{parskip}

\newcommand{\justif}[2]{&{#1}&\text{#2}}
%\newcommand{\sub}[2]{\lbrack #1/#2\rbrack}

\begin{document}

\textsc{Theorem I} ($L_{ind} \subset L_{em}$): $\forall \sigma, (\Gamma \vdash_{ind} \sigma) \implies (\Gamma \vdash_{em} \sigma)$ \\

\textsc{Proof:} \\
Proceding by induction on the derivation of $\sigma$, we observe that for every rule other than induction, Theorem I immediately holds, since these rules are shared by both $L_{ind}$ and $L_{em}$.

In the case of induction, we have: 
\begin{prooftree}
\AxiomC{$\Gamma, P(0), \forall n(P(n) \to P(S(n))) \vdash_{ind} C $}
\RightLabel{\scriptsize(Induction)}
\UnaryInfC{$\Gamma, \forall n(P(n)) \vdash_{ind} C $}
\end{prooftree}

By the inductive hypothesis, we deduce: $$\Gamma, P(0), \forall n[P(n) \to P(S(n))] \vdash_{em} C $$

To prove Theorem I, it suffices to show $\Gamma, \forall n(P(n)) \vdash_{em} C $

First, we present a proof in prose:

\begin{enumerate}
\item Suppose $P(0) \wedge \forall n(P(n) \to P(S(n)))$.
\item For the purposes of contradiction, further suppose that $\lnot\forall n(P(n))$.
\item Then, by DeMorgan's Quantifier Negation Lemma, $\exists n(\lnot P(n))$.
\item By the Infimum property of natural numbers, we then have, $$\exists n(\lnot P(n) \wedge \forall m(m<n \to \lnot\lnot P(m)))$$
\item Additionally, we conclude from \textbf{1} that $\exists n(P(n))$
\item An additional application of the Infimum property on \textbf{5} yields $$\exists n(P(n) \wedge \forall m(m<n \to \lnot P(m))$$
\item By \textbf{4} and \textbf{6}, we let N and M be such that:
$$\lnot P(M) \wedge \forall m(m<M \to \lnot\lnot P(M))$$
$$P(N) \wedge \forall m(m<N \to \lnot P(N))$$
\item By the Trichotomy Axiom, we have that 

\end{enumerate}


\end{document}
